\begin{problem}[8.4.1] \hfill

	By definition of brownian bridge,
	\[
		\begin{split}
			P\left( \max_{0 \le t \le 1} B_t ^\circ > b \right)
			&=  P_0(T_b < 1 \lvert B_1 = 0) \\
			&=  \sqrt{2\pi} P_0 \left( T_b <1, B_1 = 0 \right) \\
			&= \sqrt{2\pi} \frac{1}{\sqrt{2\pi}}\exp\left( -\frac{4b^2}{2} \right) = \exp(-2b^2)
		\end{split}
	\]
	where the third equality follows from exercise 7.4.3 (b).

	\qed
\end{problem}

\begin{problem}[8.4.2] \hfill

	We will show that two densities of them are the same.
	First,
	\[
		P\left( X_t = a \right) 
		= P\left( B_{t(1-t)} = a \right)
		= \frac{1}{\sqrt{2\pi t(1-t)}}\exp\left( -\frac{a^2}{2t(1-t)} \right)
	\]
	by Brownian scaling.

	On the other hand,
	\[
		\begin{split}
			P\left( B_t^\circ = a \right)
			&= P(B_t = a \lvert B_1 = 0) \\
			&= \sqrt{2\pi} \frac{1}{\sqrt{2\pi t}}\exp\left( -\frac{a^2}{2t} \right) \frac{1}{\sqrt{2\pi(1-t)}}\exp\left( -\frac{a^2}{2(1-t)} \right) \\
			&= \frac{1}{\sqrt{2\pi t(1-t)}} \exp\left( -\frac{a^2}{2t(1-t)} \right)
		\end{split}
	\]
	by equation (8.4.4) of our textbook.

	\qed
\end{problem}
