\begin{problem}[1.1]
\begin{equation*}
	\begin{split}
		1- \left | \frac{z-w}{1-z\overline{w}} \right | ^2 & = 1 - \frac{\left( z-w \right)\left( \overline{z} - \overline{w} \right)}{\left( 1-z\overline{w} \right)\left( 1-\overline{z}w \right)} \\
		& = \frac{1-\overline{z}w -z\overline{w} + |z|^2|w|^2 -|z|^2 - |w|^2 + z\overline{w}+\overline{z}w}{|1-\overline{z}w|^2} \\
		& = \frac{\left( 1-|z|^2 \right)\left( 1-|w|^2 \right)}{|1-\overline{z}w|^2}
	\end{split}
	\label{<+label+>}
\end{equation*}
\end{problem}

\begin{problem}[1.2] \hfill

	Let $f = u+iv$. $\partial f = \frac{1}{2} \left( \frac{\partial}{\partial x} - i\frac{\partial}{\partial y} \right)\left( u+iv \right)$.
	Then $\overline{\partial f} = \frac{1}{2}\left( \frac{\partial}{\partial x} + i\frac{\partial}{\partial y} \right)\left( u-iv \right) = \bar{\partial} \bar{f}$.
\end{problem}

\begin{problem}[1.3] \hfill

	If $f$ is constant, then $|f|$ is also constant.
	On the other hand, assume $f = u+iv$ and $|f|^2 = u^2 + v^2$ is positive real number. (if it is zero, then $f$ must be zero)
	\begin{equation*}
		u^2 + v^2 = R >0
		\label{<+label+>}
	\end{equation*}
	Differentiate both sides of the equation above with x and y respectively, we can get $uu_x +vv_x = 0$, $uu_y + vv_y = 0$, $u_x = v_y$ and $u_y = -v_x$.
	By simple calculation we can get $u_x = u_y = v_x = v_y = 0$. Therefore $u, v$ are constant.
\end{problem}

\begin{problem}[1.4] \hfill

	Note that $\int_0^{2\pi}e^{ik\theta}d\theta = \int_{0}^{2\pi}\left( \cos k\theta + i\sin k\theta \right)d\theta = 0$ for positive integer $k$. 
	Therefore $\frac{1}{2\pi} \int_{0}^{2\pi}(z_0 + re^{i\theta})^j d\theta = \frac{1}{2\pi}\int_{0}^{2\pi}\sum_{k=0}^{j}{j \choose k}z_0^k\left( re^{i\theta} \right)^{j-k}d\theta = z_0^{j}$.
	Similarly, we can get $\frac{1}{2\pi}\int_{0}^{2\pi}\overline{\left( z_0 + re^{i\theta} \right)^j}d\theta = \bar{z_0}^j$.

	Since $u$ is polynomial, we can write it as $\sum_{l, k}a_{l, k}z^l \bar{z}^k$. By direct computation, we can get $\frac{1}{2\pi}\int_{0}^{2\pi} u\left( z_0 +re^{i\theta} \right)d\theta = \sum_{l, k}a_{l, k}z_0^{l}\bar{z_0}^{k} = u(z_0)$.
	
\end{problem}

\begin{problem}[1.5] \hfill

	Let $f = u+iv$. $(g\circ f)_x = g_u u_x + g_v v_x$. Then
	\begin{equation*}
		\begin{split}
			\left( g\circ f \right)_{xx} = \left( g_{uu} u_x + g_{uv} v_x \right) u_x +g_u u_{xx} + \left( g_{vu} u_x + g_{vv} v_x \right) v_x + g_v v_{xx} \\
			\left( g\circ f  \right)_{yy} = \left( g_{uu} u_y + g_{uv }v_y \right)u_y + g_u u_{yy} + \left( g_{vu}u_y + g_{vv}v_y \right)v_y + g_v v_{yy}
		\end{split}
		\label{<+label+>}
	\end{equation*}

	But we have Cauchy-Riemann equation and $g_{uu} + g_{vv} = 0$ and $g_{vu} = g_{uv}$. Also, since $f$ is $C^2$ function, $f$ is harmonic, $u_{xy} = u_{yx}$, and $v_{xy} = v_{yx}$. Using these equations, we can check that $\left( g\circ f \right)_{xx} + \left( g \circ f \right)_{yy} = 0$. Hence $\left( g \circ f \right)$ is a harmonic function.
\end{problem}
