\begin{problem}[4.1.1] \hfill

	\[
		P(G | A) = P(A \cap G) / P(A) = \int_G 1_A dP / \int_\Omega 1_A dP = \int_g P(A|\mathcal{G})dP / \int_\Omega P(A|\mathcal{G}) dP
	\]

	\qed
\end{problem}

\begin{problem}[4.1.2]\hfill

	Let $A \in \mathcal{F}$.
	Then
	\[
		a^2 \int_A 1_{(|X| \geq a)}dP \leq \int_A X^2 1_{(|X| \geq a)}dP \leq \int_A X^2 dP
	\]
	which leads
	\[
		a^2 P(|X| \geq a | \mathcal{F}) \leq E(X^2 | \mathcal{F}).
	\]

\qed	
\end{problem}

\begin{problem}[4.1.3]\hfill

	Let $\theta$ be any real number.
	Then
	\[
		E\left( (X+\theta Y)^2 | \mathcal{G} \right) \geq 0.
	\]
	
	By linearity of conditional expectation, we get
	\[
		E(X^2 |\mathcal{G}) + 2\theta E(XY | \mathcal{G}) + \theta^2 E(Y^2 | \mathcal{G}) \geq 0.
	\]

	Thus, the conclusion follows.

	\qed
	
\end{problem}

\begin{problem}[4.1.5] \hfill

	Let $P(a) = P(b) = P(c) = 1/3$, $X = 1_{(a)}$, $\mathcal{F}_1 = \sigma(\{a\})$, and $\mathcal{F}_2 = \sigma(\{b\})$.
	Then
	\[
		E(X | \mathcal{F}_2) = \frac{1}{2} 1_{\{a, c\}}
	\]
	but
	\[
		E\left( E(X |\mathcal{F}_2) | \mathcal{F}_1 \right) = \frac{1}{3}1_{(a)} + \frac{1}{4}1_{\{b, c\}}.
	\]

	\qed
	
\end{problem}

\begin{problem}[4.1.6] \hfill

	Note that
	\[
		\int E(X|\mathcal{F})^2 dP = \int E(X E(X|\mathcal{F}) | \mathcal{F}) dP = \int X E(X |\mathcal{F}) dP.
	\]
	Use the above.

	\qed
	
\end{problem}

\begin{problem}[4.1.7] \hfill

	By definition of $\Var (X | \mathcal{F})$, we get the following:
\[
	E \left( \Var (X | \mathcal{F} ) \right) = EX^2 - E\left( E(X|\mathcal{F})^2 \right)
\]
	And clearly,
\[
	\Var \left( E(X|\mathcal{F}) \right) = E\left( E(X|\mathcal{F})^2 \right) - \left( E( E(X|\mathcal{F}) ) \right)^2
\]

Therefore, by summing them vertically, we can get
\[
	\Var \left( E(X|\mathcal{F}) \right) + E\left( \Var(X|\mathcal{F} \right) = EX^2 - \left( E(E(X|\mathcal{F})) \right)^2
\]
which is equal to $\Var(X)$ since the last term is equal to square of $EX$.
\qed
\end{problem}

\begin{problem}[4.1.9] \hfill
\[
	\begin{split}
		\int |X-Y|^2 dP
		& = \int X^2 - 2XY + Y^2 dP \\
		& = \int X^2 - 2E(XY | \mathcal{G}) +Y^2 dP \\
		& = \int X^2 -2X E(Y|\mathcal{G}) +Y^2 dP \\
		& = \int X^2 - 2X^2 + Y^2 dP \\
		& = EY^2 - EX^2 \\
		& = 0
	\end{split}
\]
Therefore, $|X-Y|^2 = 0$ a.s. which implies $X = Y$ a.s.
Note that $XY$ is integrable by Holder's inequality for $p = q = 2$ and finite second moment of $X, Y$.
\qed
\end{problem}

\begin{problem}[4.1.10]\hfill

	Let $Z= E(X |\mathcal{G})$.
	\[
		\begin{split}
			EX^+ - EX^- & = EX = EZ = EZ^+ - EZ^- \\
			& = \int_{Z>0}Z dP + \int_{Z<0} ZdP \\
			& = \int_{Z>0}X dP + \int_{Z<0} XdP
		\end{split}
	\]
	also,
	\[
		\begin{split}
			EX^+ +EX^- & = E|X| = E|Z| = EZ^+ +EZ^- \\
			& = \int_{Z>0}Z dP - \int_{Z<0}Z dP \\
			& = \int_{Z>0}X dP - \int_{Z<0}X dP
		\end{split}
	\]
	thus
	\[
		\int X^+ -1_{Z>0}X dP = 0.
	\]
	But, from $X^+ \geq 1_{Z>0}X$, we can catch $X^+ = 1_{Z>0}X$ almost surely.
	Similarly, $X^- = -1_{Z<0}X$ almost surely.
	Therefore each sign functions of $X$ and $E(X|\mathcal{G})$ are equal almost surely.
	
	Now consider
	\[
		\left\{ Y < E(Y |\mathcal{G}) \right\} = \bigcup_{i\in \mathbb{N}}\left\{ Y < q_i < E(Y|\mathcal{G}) \right\}
			= \bigcup_{i\in \mathbb{N}}B_i
	\]
	where $q_i$'s are enumeration of the rationals.

	Note that $B_i = \left\{ Y - q_i <0 \right\} \cap \left\{ E(Y|\mathcal{G}) - q_i > 0 \right\}$.
	But, by using the fact that each sign functions of $Y - q_i$ and $E(Y|\mathcal{G}) - q_i$ are equal almost surely,
	we get
	\[
		P(B_i) = 0
	\]
	for each $i\in \mathbb{N}$.
	Thus $P(Y <E(Y|\mathcal{G}) ) = 0$.

	By similar assertion, $Y = E(Y|\mathcal{G})$ almost surely.

	\qed
\end{problem}
\begin{problem}[4.2.3] \hfill

	Clearly $\mathcal{F}_m \subset \mathcal{F}_{m+1}$ for all positive integer $m$.
	Let $Z_n = X_n \vee Y_n$, then $Z_n$ is clearly $\mathcal{F}_n$ measurable.
	
	Now, let $A \in \mathcal{F}_{n-1}$. Then,
\[
	\begin{split}
		\int_A E(Z_n | \mathcal{F}_{n-1}) dP
		& = \int_A Z_n dP \\
		& \geq \int_A X_n dP \vee \int_A Y_n dP \\ 
		& = \int_A E(X_n | \mathcal{F}_{n-1})dP \vee \int_A E(Y_n | \mathcal{F}_{n-1}) dP \\
		& \geq \int_A X_{n-1} dP \vee \int_A Y_{n-1} dP
	\end{split}
\]
Therefore $\int_A E(Z_n | \mathcal{F}_{n-1}) dP \geq \int_A X_{n-1}, Y_{n-1} dP$ for all $A \in \mathcal{F}_{n-1}$.
Since $E(Z_n | \mathcal{F}_{n-1})$ is $\mathcal{F}_{n-1}$ measurable, we can conclude that conditional expectation of $Z_n$ with respect to $\mathcal{F}_{n-1}$ is equal or greater than $X_{n-1}$ and $Y_{n-1}$ a.s.

So, $Z_n$ is a submartingale.
\qed
\end{problem}

\begin{problem}[4.2.9] \hfill

	Note that $\left\{ N > n \right\} = \left\{ N \leq n \right\}^c \in \mathcal{F}_{n}$ and $\left\{ N<n \right\} = \left\{ N \leq n-1 \right\} \in \mathcal{F}_{n-1}$ since $N$ is integer valued. 
	Now, consider the following:

\[
	\begin{split}
		E(Z_n | \mathcal{F}_{n-1})
		& = 1_{N \geq n} E(X_n^1 | \mathcal{F}_{n-1}) + 1_{N < n} E(X_n^2 |\mathcal{F}_{n-1}) \\
		& \leq 1_{N \geq n} X_{n-1}^1 + 1_{N<n}X_{n-1}^2 \\
		& = 1_{N > n-1} X_{n-1}^1 + 1_{N \leq n-1} X_{n-1}^2 \\
		& \leq 1_{N \geq n-1} X_{n-1}^1 + 1_{N < n-1} X_{n-1}^2 \\
		& = Z_{n-1}
	\end{split}
\]
So, $Z_n$ is supermartingale.

	Now, consider the $Y_n$:
	
	First, $Y_n = X_n^1 1_{N>n} + X_N^2 1_{N=n} + X_n^2 1_{N<n} \leq X_n^1 1_{N\geq n} + X_n^2 1_{N <n}$.
\[
	\begin{split}
		E(Y_n |\mathcal{F}_{n-1})
		& \leq 1_{N\geq n} E\left( X_n^1 | \mathcal{F}_{n-1} \right) + !_{N<n}E\left( X_n^2 | \mathcal{F}_{n-1} \right) \\
		& \leq 1_{N \geq n} X_{n-1}^1 + 1_{N < n}X_{n-1}^2 \\
		& = 1_{N > n-1} X_{n-1}^1 + 1_{N \leq n-1}X_{n-1}^2 \\
		& = Y_{n-1}
	\end{split}
\]
So, $Y_n$ is also a supermartingale. \qed
\end{problem}
