\section{2020.08}

\begin{problem}
	Use the following formula:
	\[
		\int_{(a, b]}G dF+F dG = F(b)G(b)-F(a)G(a) + \sum_{x \in (a, b]}\left( F(x) - F(x^-) \right).
	\]
	Note that the last term is the sum of atoms.

	In our case, $G(x) = x^3$.

	\qed
\end{problem}

\begin{problem}
	\[
		\frac{\sum X_k}{\sqrt{\sum X_k^2}} = \frac{\sum X_k / n}{\sigma / \sqrt{n}} \frac{\sigma}{\sqrt{\sum X_k^2 /n}}
	\]
	Now apply the Central limit theorem, law of large numbers, and Slutsky's theorem.

	\qed
\end{problem}

\begin{problem}
	Let $X_i$'s are iid random variables which follow exponential distribution of rate $2$.
	Then given integral is equal to
	\[
		\mathbb{E}\cos\left( \frac{X_1 + \cdots X_n}{n} \right).
	\]
	By law of large numbers,
	\[
		\frac{X_1 + \cdots X_n}{n} \rightarrow _p \mathbb{E}X_1 = \frac{1}{2}.
	\]
	Since $\cos$ is bounded continuous function, by applying bounded convergence theorem, given limit is equal to $\cos1/2$.

	\qed
\end{problem}

\begin{problem}
	Observe that $S_n$ is a martingale.
	Thus $|S_n|^2$ is a submartingale, and we will apply Doob's inequality.

	Let $A = \left\{ \max_{1 \leq k \leq n}|S_k|^2 \geq \lambda^2 \right\}$.
	Then by Doob's inequality,
	\[
		\lambda^2 P(A) \leq \mathbb{E}S_n^2 1_{A} \leq \mathbb{E}|S_n|^2 = \Var{S_n}.
	\]
	But $A = \left\{ \max_{1\leq k\leq n}|S_k| \geq \lambda \right\}$.
	Therefore we get the result.

	\qed
\end{problem}

\begin{problem}
	Consider the corresponding quadratic martingale $M_n = S_n^2 - n\sigma^2 = S_n^2 -n$.
	Then $M_{n\wedge T}$ is also a martingale.
	Thus, $\mathbb{E} M_{n\wedge T} = \mathbb{E}M_0 = 0$ implies
	\[
		\mathbb{E} S_{n\wedge T}^2 = \mathbb{E} n\wedge T.
	\]
	But the right hand side goes to $\mathbb{E} T$ by monotone convergence theorem.
	And note that
	\[
		| S_{n\wedge T} | \leq \max( |a|, |b| ).
	\]
	Thus bounded convergence theorem implies $\mathbb{E} S_{n\wedge T}^2 \rightarrow \mathbb{E}S_T^2$. 
	\[
		\mathbb{E} S_T^2 = P(S_T = a) a^2 + P(S_T = b) b^2 = (x-a)(b-x)
	\]
	To complete the above, we must show that $T<\infty$ a.s.
	This can be done by considering
	\[
		P\left( T > m(b-a) \right) \leq \left( 1- \left( 1/2 \right)^{b-a} \right)^m.
	\]

	\qed
\end{problem}
